Distinguish between switches and hosts

src/mininet-topology.py
@@ -2,46 +2,51 @@
 
 from mininet.topo import Topo
 
+# Run on a mininet VM with:
+# sudo mn --custom src/mininet-topology.py --topo mytopo --arp --mac --controller=remote,ip=<controller IP>,port=6633
+
 class MyTopo(Topo):
 	def __init__(self):
 		Topo.__init__(self)
-		A = self.addSwitch('s1')
-		aHost = self.addHost('h1')
-		B = self.addSwitch('s2')
-		bHost = self.addHost('h2')
-		C = self.addSwitch('s3')
-		cHost = self.addHost('h3')
-		D = self.addSwitch('s4')
-		dHost = self.addHost('h4')
-		E = self.addSwitch('s5')
-		eHost = self.addHost('h5')
-		F = self.addSwitch('s6')
-		fHost = self.addHost('h6')
+		sA = self.addSwitch('s1')
+		hA = self.addHost('h1')
+		sB = self.addSwitch('s2')
+		hB = self.addHost('h2')
+		sC = self.addSwitch('s3')
+		hC = self.addHost('h3')
+		sD = self.addSwitch('s4')
+		hD = self.addHost('h4')
+		sE = self.addSwitch('s5')
+		hE = self.addHost('h5')
+		sF = self.addSwitch('s6')
+		hF = self.addHost('h6')
 
-		self.addLink(aHost, A, 0, 99)
-		self.addLink(bHost, B, 0, 99)
-		self.addLink(cHost, C, 0, 99)
-		self.addLink(dHost, D, 0, 99)
-		self.addLink(eHost, E, 0, 99)
-		self.addLink(fHost, F, 0, 99)
-
+		#
 		# example_topology:
-		#      B ------> E
-		#    / | \       ↑
-		#   A  |  D <--- F
-		#    \ | /
-		#      C
+
+		#    hB --- sB ----> sE      hE
+		#          / | \   /          |
+		# hA --- sA  |  sD ---- sF ---|
+		#         \  | /   \      ↖______- hF
+		#           sC - hC \__- hD
 
 		# Note: This network is more lenient than the diagram above in that
-		# all links are bidirectional.
+		# all links are bidirectional. For easier debugging, directed edges
+		# that are not present in the model topology have port number 1000.
 
-		self.addLink(A, B, 1, 1)
-		self.addLink(A, C, 2, 1)
-		self.addLink(B, C, 2, 2)
-		self.addLink(B, D, 3, 1)
-		self.addLink(B, E, 4, 1000)
-		self.addLink(C, D, 3, 2)
-		self.addLink(F, D, 1, 1000)
-		self.addLink(E, F, 1, 2)
+		self.addLink(hA, sA, 1, 1)
+		self.addLink(sA, sB, 2, 1)
+		self.addLink(sA, sC, 3, 1)
+		self.addLink(hB, sB, 1, 2)
+		self.addLink(sB, sC, 3, 2)
+		self.addLink(sB, sD, 4, 1)
+		self.addLink(sB, sE, 5, 1000)
+		self.addLink(hC, sC, 1, 3)
+		self.addLink(sC, sD, 4, 2)
+		self.addLink(hD, sD, 1, 3)
+		self.addLink(sD, sE, 4, 1)
+		self.addLink(sD, sF, 5, 1)
+		self.addLink(hE, sF, 1, 2)
+		self.addLink(hF, sF, 1, 1000)
 
 topos = {'mytopo': lambda: MyTopo()}
